\documentclass[11pt,letterpaper]{article}
\usepackage[lmargin=1in,rmargin=1in,bmargin=1in,tmargin=1in]{geometry}
\usepackage{checkins}

\DeclareMathOperator{\arccot}{arccot}
\newcommand{\boxseven}[4]{%
	\draw[thick] (0,0) -- (4,0) -- (4,4) -- (0,4) -- (0,0);
	\draw[thick] (0,2) -- (4,2);
	\draw[thick] (2,0) -- (2,4);
	% '7'
	\draw (1.7,2.2) -- (2.3,2.2) -- (1.7,1.6);
	% Entries
	\node at (1,3) {$#1$};	% u
	\node at (3,1) {$#2$};	% dv
	\node at (1,1) {$#3$};	% du
	\node at (3,3) {$#4$};	% 
}

\usetikzlibrary{calc}
\usepackage{booktabs}
\tikzset{Arrow Style/.style={text=black, font=\boldmath}}
\newcommand{\tikzmark}[1]{%
    \tikz[overlay, remember picture, baseline] \node (#1) {};%
}
\newcommand*{\XShift}{0.5em}
\newcommand*{\YShift}{0.5ex}
\NewDocumentCommand{\DrawArrow}{s O{} m m m}{%
    \begin{tikzpicture}[overlay,remember picture]
        \draw[->, thick, Arrow Style, #2] 
                ($(#3.west)+(\XShift,\YShift)$) -- 
                ($(#4.east)+(-\XShift,\YShift)$)
        node [midway,above] {#5};
    \end{tikzpicture}%
}
\usepackage{polynom}




% -------------------
% Content
% -------------------
\begin{document}
\thispagestyle{title}

% 01/16
\checkin{01/16} Given $\ds\int_0^\pi e^{\sin x} \cos x \;dx$, the $u$-substitution $u= \sin x$ transforms this integral into $\ds\int_0^\pi e^u \;du$. \pspace

\sol The statement is \textit{false}. If $u= \sin x$, then $du= \cos x \,dx$. So indeed, this $u$-substitution would transform the integral $\ds\int e^{\sin x} \cos x \,dx$ into the integral $\ds\int e^u \,du$. However with definite integrals, one needs to remember to transform the limits as well. If $x= 0$, then $u= \sin(0)= 0$. If $x= \pi$, then $u= \sin(\pi)= 0$. Therefore, the correct substitution is $\ds\int_0^\pi e^{\sin x} \cos x \,dx= \int_0^0 e^u \,du= 0$. \pvspace{1.3cm}



% 01/21
\checkin{01/21} To integrate $\ds\int \arccot \theta \,d\theta$, one can use integration-by-parts by choosing $u= \arccot \theta$ and $dv= 1$. \pspace

\sol The statement is \textit{true}. Using LIATE, it is likely that the choice of $u= \arccot \theta$ will work. With `nothing left' in the integrand, this means that $dv= 1$. We fill in our box as follows:
	\[
	\begin{tikzpicture}
	% Left Boxes
	\draw[thick] (0,0) -- (4,0) -- (4,4) -- (0,4) -- (0,0);
	\draw[thick] (0,2) -- (4,2);
	\draw[thick] (2,0) -- (2,4);
	% Entries
	\node at (1,3) {$\arccot \theta$};	% u
	\node at (3,1) {$1$};				% dv
	
	\tikzset{shift={(3,0)}}
	
	\node at (2,2) {\scalebox{1.5}{$\Longrightarrow$}};
	
	\tikzset{shift={(3,0)}}
	
	\boxseven{\arccot \theta}{1}{\dfrac{-1}{1 + \theta^2}}{\theta}
	\end{tikzpicture}
	\]
Then using the `Rule of 7', we find that\dots
	\[
	\int \arccot \theta \,d\theta= \theta \arccot \theta - \int \dfrac{-\theta}{1 + \theta^2} \,d\theta= \theta \arccot \theta + \int \dfrac{\theta}{1 + \theta^2} \,d\theta
	\]
Using the $u$-substitution $u= 1 + \theta^2$, we see that $\ds\int \frac{\theta}{1 + \theta^2} \,d\theta= \frac{1}{2} \ln|1 + \theta^2| + C$. Therefore, we have\dots
	\[
	\int \arccot \theta \,d\theta= \theta \arccot \theta + \dfrac{1}{2} \ln|1 + \theta^2| + C
	\] \pvspace{1.3cm}



% 01/23
\checkin{01/23} The integral $\ds\int e^{x/2} \sin(3x) \;dx$ is a `looping' integral. \pspace

\sol The statement is \textit{true}. Recall that integrals whose integrand is the product of an exponential function with $\sin x$ or $\cos x$ `loop.' We can see this directly: choose $u= \sin(3x)$. Using the `box method', we have\dots
	\[
	\begin{tikzpicture}
	\boxseven{\sin(3x)}{e^{x/2}}{3 \cos(3x)}{2e^{x/2}}
	\end{tikzpicture}
	\]
Therefore, we have\dots
	\[
	\int e^{x/2} \sin(3x) \;dx= 2 e^{x/2} \sin(3x) - \int 6e^{x/2} \cos(3x) \;dx
	\]
But this integral on the right also requires integration-by-parts: we choose $u= \cos(3x)$ and then\dots
	\[
	\begin{tikzpicture}
	\boxseven{\cos(3x)}{6 e^{x/2}}{-3 \sin(3x)}{12 e^{x/2}}
	\end{tikzpicture}
	\]
So then we have\dots
	\[
	\begin{aligned}
	\int e^{x/2} \sin(3x) \;dx&= 2 e^{x/2} \sin(3x) - \int 6e^{x/2} \cos(3x) \;dx \\
	&= 2 e^{x/2} \sin(3x) - \left(12 e^{x/2} \cos(3x) - \int -36 e^{x/2} \sin(3x) \;dx \right) \\
	&= 2 e^{x/2} \sin(3x) - 12 e^{x/2} \cos(3x) + \int -36 e^{x/2} \sin(3x) \;dx \\
	&= 2 e^{x/2} \sin(3x) - 12 e^{x/2} \cos(3x) - 36 \int e^{x/2} \sin(3x) \;dx
	\end{aligned}
	\]
Observe that we have `looped'---obtaining a multiple of the original integral on the right. Adding $\ds 36 \int e^{x/2} \sin(3x) \;dx$ to both sides, we have\dots
	\[
	37 \int e^{x/2} \sin(3x) \;dx= 2 e^{x/2} \sin(3x) - 12 e^{x/2} \cos(3x)
	\]
Therefore, we have\dots
	\[
	\int e^{x/2} \sin(3x) \;dx= \dfrac{2 e^{x/2} \sin(3x) - 12 e^{x/2} \cos(3x)}{37} + C
	\]
We can shortcut this work by adjusting tabular integration: 
	\[
	\renewcommand{\arraystretch}{1.5}
	\begin{array}{c @{\hspace*{1.3cm}} c} \toprule
	u & dv \\ \cmidrule(lr){1-2}
	\sin(3x) \tikzmark{Left 1} & \tikzmark{Right 1} e^{x/2} \\[0.3cm]
	3 \cos(3x) \tikzmark{Left 2} & \tikzmark{Right 2} 2 e^{x/2} \\[0.3cm]
	-9 \sin(3x) \tikzmark{Left 3}  & \tikzmark{Right 3} 4 e^{x/2} 
	
	\DrawArrow{Left 1}{Right 2}{+}
	\DrawArrow{Left 2}{Right 3}{--}
	\DrawArrow{Left 3}{Right 3}{+}
	\end{array}
	\]
Therefore, we have\dots
	\[
	\begin{aligned}
	\int e^{x/2} \sin(3x) \;dx&= 2 e^{x/2} - 12 e^{x/2} \cos(3x) - 36 \int e^{x/2} \sin(3x) \; dx \\
	37 \int e^{x/2} \sin(3x) \;dx&= 2 e^{x/2} - 12 e^{x/2} \cos(3x) \\
	\int e^{x/2} \sin(3x) \;dx&= \dfrac{2 e^{x/2} \sin(3x) - 12 e^{x/2} \cos(3x)}{37} + C
	\end{aligned}
	\] \pvspace{1.3cm}



% 01/28
\checkin{01/28} To integrate $\ds\int \cos^8 \theta \sin^5 \theta \;d\theta$, one should choose $u= \cos \theta$. \pspace

\sol The statement is \textit{true}. Observe that if we choose $u= \cos \theta$, then $\cos^8 \theta$ becomes $u^8$. We know $du$ will then produce a $\sin \theta$---specifically $-\sin \theta$. This `uses' one of the $\sin \theta$'s in the integrand. This leaves $\sin^4 \theta$ remaining in the integrand. But we can replace even powers of $\sin \theta$ in terms of $\cos \theta$. So we can carry out this substitution. Observe that if $u= \cos \theta$, then $du= -\sin \theta \;d\theta$. But then using the fact that $\sin^2 \theta= 1 - \cos^2 \theta$ (so that $\sin^4 \theta= (\sin^2 \theta)^2= (1 - \cos^2 \theta)^2$), we have\dots
	\[
	\begin{aligned}
	\int \cos^8 \theta \sin^5 \theta \;d\theta&= \int \cos^8 \theta \sin^4 \theta \cdot \sin \theta \; d\theta \\
	&= -\int \cos^8 \theta \sin^4 \theta \cdot -\sin \theta \; d\theta \\
	&= -\int \cos^8 \theta (1 - \cos^2 \theta)^2 \cdot -\sin \theta \;d\theta \\
	&= -\int u^8 (1 - u^2)^2 \;du \\
	&= -\int u^8 (1 - 2u^2 + u^4) \;du \\
	&= \int -u^8 + 2u^{10} - u^{12} \;du \\
	&= -\dfrac{u^9}{9} + \dfrac{2u^{11}}{11} - \dfrac{u^{13}}{13} + C \\
	&= -\dfrac{\cos^9 \theta}{9} + \dfrac{2\cos^{11} \theta}{11} - \dfrac{\cos^{13} \theta}{13} + C
	\end{aligned}
	\]
Alternatively, observe that if we had chosen $u= \sin \theta$, then $\sin^5 \theta$ becomes $u^5$. We know that $du$ produces a $\cos \theta$. This `uses' one of the $\cos \theta$'s in the integrand. This leaves $\cos^7 \theta$ remaining in the integrand. However, we can only replace even powers of $\cos \theta$ in terms of $\sin \theta$ using $\cos^2 \theta= 1 - \sin^2 \theta$. So without using other identities or using other techniques, we cannot `simply' choose $u= \sin \theta$ for this integral. \pvspace{1.3cm}



% 01/30
\checkin{01/30} To compute $\ds\int \dfrac{x^3}{\sqrt{x^2 - 4}} \;dx$, one can make the substitution $x= 2 \sec \theta$. \pspace

\sol The statement is \textit{true}. Observe we have the term $x^2 - 4$, which resembles a term from the Pythagorean Theorem. For a right triangle, we know that $a^2 + b^2= c^2$. This implies that $a^2= c^2 - b^2$, which is $x^2 - 4$ if $c^2= x^2$ and $b^2= 4$, i.e. $c= x$ and $b= 2$. We construct a triangle with $c= x$ and $b= 2$. This only gives two possibilities:
	\[
	\begin{tikzpicture}
	\draw[line width=0.03cm] (0,0) -- (1.5,0) -- (1.5,2) -- (0,0);
	\draw[line width=0.02cm] (1.3,0) -- (1.3,0.2) -- (1.5,0.2);
	\node at (0.45,0.25) {$\theta$};
	\node at (0.55,1.1) {$x$};
	\node at (0.75,-0.3) {$2$};
	
	\tikzset{shift={(4,0)}}

	\draw[line width=0.03cm] (0,0) -- (1.5,0) -- (1.5,2) -- (0,0);
	\draw[line width=0.02cm] (1.3,0) -- (1.3,0.2) -- (1.5,0.2);
	\node at (0.45,0.25) {$\theta$};
	\node at (0.55,1.1) {$x$};
	\node at (1.8,0.9) {$2$};
	\end{tikzpicture}
	\]
In the first, we would have $\cos \theta= \frac{2}{x}$, which implies that $x= \frac{2}{\cos \theta}= 2 \sec \theta$. This is the given substitution. In the second, we would have $\sin \theta= \frac{2}{x}$, which implies that $x= \frac{2}{\sin \theta}= 2 \csc \theta$. 

Choosing the former substitution, we would have $x= 2 \sec \theta$, so that $dx= 2 \sec \theta \tan \theta$. Calling the vertical side $s$ and using the Pythagorean Theorem, we see that $2^2 + s^2= x^2$, i.e. $4 + s^2= x^2$. But then $s= \sqrt{x^2 - 4}$. This gives us the following triangle: 
	\[
	\begin{tikzpicture}
	\draw[line width=0.03cm] (0,0) -- (1.5,0) -- (1.5,2) -- (0,0);
	\draw[line width=0.02cm] (1.3,0) -- (1.3,0.2) -- (1.5,0.2);
	\node at (0.45,0.25) {$\theta$};
	\node at (0.55,1.1) {$x$};
	\node at (0.75,-0.3) {$2$};
	\node at (2.4,0.9) {$\sqrt{x^2 - 4}$};
	\end{tikzpicture}
	\]
We need to find $x^3$ and $\sqrt{x^2 - 4}$. Because $x= 2 \sec \theta$, we know that $x^3= (2 \sec \theta)^3= 2^3 \sec^3 \theta$. To find $\sqrt{x^2 - 4}$, observe that $\tan \theta= \frac{\sqrt{x^2 - 4}}{2}$, which implies that $\sqrt{x^2 - 4}= 2 \tan \theta$. Therefore, we have\dots
	\[
	\int \dfrac{x^3}{\sqrt{x^2 - 4}} \;dx= \int \dfrac{2^3 \sec^3 \theta}{2 \tan \theta} \cdot 2 \sec \theta \tan \theta \;d\theta= \int 8 \sec^4 \theta \;d\theta
	\]
Now using the fact that $\tan^2 \theta + 1= \sec^2 \theta$, we know that 
	\[
	\sec^4 \theta= (\sec^2 \theta)^2= (\tan^2 \theta + 1)^2= \tan^4 \theta + 2 \tan^2 \theta + 1
	\]
But then\dots
	\[
	\int 8 \sec^4 \theta \;d\theta= \int 8 \sec^2 \theta \sec^2 \theta \;d\theta= \int 8 \sec^2 \theta (\tan^2 \theta + 1) \;d\theta= \int 8(\tan^2 \theta + 1) \cdot \sec^2 \theta \;d\theta
	\]
Now letting $u= \tan \theta$, we have $du= \sec^2 \theta \;d\theta$. But then\dots
	\[
	\int 8(\tan^2 \theta + 1) \cdot \sec^2 \theta \;d\theta= \int 8(u^2 + 1) \;du= 8 \int (u^2 + 1) \;du= 8 \left( \dfrac{u^3}{3} + u \right) + C
	\]
Replacing $u$, we have\dots
	\[
	8 \left( \dfrac{u^3}{3} + u \right) + C= 8 \left( \dfrac{\tan^3 \theta}{3} + \tan \theta \right) + C
	\]
But from the triangle, we know that $\tan \theta= \frac{\sqrt{x^2 - 4}}{2}$. Therefore, we have\dots
	\[
	8 \left( \dfrac{\tan^3 \theta}{3} + \tan \theta \right) + C=. 8 \left( \dfrac{1}{3} \cdot \left( \dfrac{\sqrt{x^2 - 4}}{2} \right)^3 + \dfrac{\sqrt{x^2 - 4}}{2} \right) + C
	\]
If we simplify this, we have\dots
	\[
	\begin{gathered}
	8 \left( \dfrac{1}{3} \cdot \left( \dfrac{\sqrt{x^2 - 4}}{2} \right)^3 + \dfrac{\sqrt{x^2 - 4}}{2} \right) + C \\
	8 \cdot \dfrac{\sqrt{x^2 - 4}}{2} \left( \dfrac{1}{3} \cdot \left( \dfrac{\sqrt{x^2 - 4}}{2} \right)^2 + 1 \right) + C \\
	4 \sqrt{x^2 - 4} \left( \dfrac{1}{3} \cdot \dfrac{x^2 - 4}{4} + 1 \right) + C \\
	4 \sqrt{x^2 - 4} \left( \dfrac{x^2 - 4}{12} + 1 \right) + C \\
	4 \sqrt{x^2 - 4} \left( \dfrac{x^2 - 4}{12} + \dfrac{12}{12} \right) + C \\
	4 \sqrt{x^2 - 4} \left( \dfrac{x^2 + 8}{12}\right) + C \\
	\dfrac{1}{3}\, \sqrt{x^2 - 4}\; (x^2 + 8) + C
	\end{gathered}
	\]
Therefore, we have\dots
	\[
	\int \dfrac{x^3}{\sqrt{x^2 - 4}} \;dx= \dfrac{1}{3}\, \sqrt{x^2 - 4}\; (x^2 + 8) + C
	\] \pvspace{1.3cm}



% 02/04
\checkin{02/04} The rational function $\dfrac{x^6 - 4x}{(x - 1)(x + 2)(x^2 + 4)}$ can be decomposed as $\dfrac{A}{x - 1} + \dfrac{B}{x + 2} + \dfrac{Cx + D}{x^2 + 4}$. \pspace

\sol The statement is \textit{false}. We know that given a rational function has a partial fraction decomposition given in the `traditional' way so long as the degree of the numerator is \textit{less} than the degree of the denominator. Observe that the degree of the numerator in the original function is 6 while the degree of the denominator is $1 + 1 + 2= 4$. So, this cannot be broken down in the `traditional' way. Alternatively, find the common denominator of $(x - 1)(x + 2)(x^2 + 4)$ for the given decomposition, observe that the numerator will have at most degree 4, which could not possibly yield the numerator of $x^6 - 4x$ with degree 6. One would first need to long divide $x^6 - 4x$ by $(x - 1)(x + 2)(x^2 + 4)$ to find the quotient and remainder before trying to give a partial fraction decomposition. Observe\dots
	\[
	(x - 1)(x + 2)(x^2 + 4)= (x^2 + x - 2)(x^2 + 4)= x^4 + x^3 + 2x^2 + 4x - 8
	\]
But then\dots
	\[
	\polylongdiv{x^6 - 4x}{x^4 + x^3 + 2x^2 + 4x - 8}
	\]
Therefore, we have\dots
	\[
	\dfrac{x^6 - 4x}{(x - 1)(x + 2)(x^2 + 4)}= x^2 - x - 1 + \dfrac{-x^3 + 14x^2 - 8x - 8}{x^4 + x^3 + 2x^2 + 4x - 8}= x^2 - x - 1 + \dfrac{-x^3 + 14x^2 - 8x - 8}{(x - 1)(x + 2)(x^2 + 4)}
	\]
We can then find the `traditional' partial fraction decomposition of the resulting rational function above because the degree of the numerator, which is 3, is \textit{less} than the degree of the denominator, which is 4. We would have\dots
	\[
	\dfrac{-x^3 + 14x^2 - 8x - 8}{(x - 1)(x + 2)(x^2 + 4)}= \dfrac{A}{x - 1} + \dfrac{B}{x + 2} + \dfrac{Cx + D}{x^2 + 4}
	\]
Using Heaviside's Method/Cover-Up Method, we can find $A$ and $B$ `instantly':
	\[
	\begin{aligned}
	A&= \dfrac{-1^3 + 14(1^2) - 8(1) - 8}{(1 + 2)(1^2 + 4)}= -\dfrac{3}{15}= -\dfrac{1}{5} \\[0.2cm]
	B&= \dfrac{-(-2^3) + 14(-2)^2 - 8(-2) - 8}{(-2 - 1) \big( (-2)^2 + 4 \big)}= \dfrac{72}{-24}= -3
	\end{aligned}
	\]
To find $C, D$, we can get a common denominator:
	\[
	\dfrac{A}{x - 1} + \dfrac{B}{x + 2} + \dfrac{Cx + D}{x^2 + 4}= \dfrac{A(x + 2)(x^2 + 4) + B(x - 1)(x^2 + 4) + (Cx + D)(x - 1)(x + 2)}{(x - 1)(x + 2)(x^2 + 4)}
	\]
Using the fact that the rational functions now have equal denominators, we can equate their numerators:
	\[
	\begin{aligned}
	-x^3 + 14x^2 - 8x - 8&= A(x + 2)(x^2 + 4) + B(x - 1)(x^2 + 4) + (Cx + D)(x - 1)(x + 2) \\[0.2cm]
	-x^3 + 14x^2 - 8x - 8&=-\frac{1}{5}\, (x + 2)(x^2 + 4) - 3(x - 1)(x^2 + 4) + (Cx + D)(x - 1)(x + 2) \\
	\end{aligned}
	\]
We multiply the last equation by 5 to clear fractions:
	\[
	5(-x^3 + 14x^2 - 8x - 8)= -(x + 2)(x^2 + 4) - 15(x - 1)(x^2 + 4) + 5(Cx + D)(x - 1)(x + 2)
	\]
Rather than expand this and relate coefficients to obtain a system of equations, we will simply substitute two $x$-values (ones not used in Heaviside's Method): using $x= 0$, we have\dots
	\[
	\begin{aligned}
	5(-x^3 + 14x^2 - 8x - 8)&= -(x + 2)(x^2 + 4) - 15(x - 1)(x^2 + 4) + 5(Cx + D)(x - 1)(x + 2) \\
	-40&= 52 - 10D \\
	-92&= -10 D \\
	\dfrac{46}{5}&= D
	\end{aligned}
	\]
and using $x= -1$ and the value for $D$ above, we have\dots
	\[
	\begin{aligned}
	5(-x^3 + 14x^2 - 8x - 8)&= -(x + 2)(x^2 + 4) + 15(x - 1)(x^2 + 4) + 5(Cx + D)(x - 1)(x + 2) \\
	75&= 145 - 10 (-C + D) \\
	-70&= 10C - 10D \\
	-70&= 10C - 10 \cdot \dfrac{46}{5} \\
	-70&= 10C - 92 \\
	22&= 10C \\
	\dfrac{11}{5}&= C
	\end{aligned}
	\]
Therefore, we have\dots
	\[
	\dfrac{x^6 - 4x}{(x - 1)(x + 2)(x^2 + 4)}= x^2 - x - 1 + \dfrac{-1/5}{x - 1} + \dfrac{-3}{x + 2} + \dfrac{\frac{11}{5}\,x + \frac{46}{5}}{x^2 + 4}= x^2 - x - 1 - \dfrac{1}{5(x - 1)} - \dfrac{3}{x + 2} + \dfrac{11x + 46}{5(x^2 + 4)}
	\] \pvspace{1.3cm}



% 02/06
\checkin{02/06} $\ds\int \dfrac{5}{x + 1} - \dfrac{1}{(x + 1)^2} - \dfrac{x + 1}{x^2 + 1} \;dx= 5 \ln(x + 1) - \dfrac{1}{x + 1} - \frac{1}{2} \ln|x^2 + 1| + \arctan x + K$ \pspace

\sol The statement is \textit{false}. First, we know that\dots
	\[
	\int \dfrac{5}{x + 1} \;dx= 5 \ln|x + 1| + K
	\]
The integral of the second term is also incorrect:
	\[
	\int -\dfrac{1}{(x + 1)^2} \;dx= \int -(x + 1)^{-2} \;dx= \dfrac{-(x + 1)^{-1}}{-1} + K= \dfrac{1}{x + 1} + K
	\]
Moreover, the third term is also incorrect as the negative has been improperly distributed:
	\[
	- \int \dfrac{x + 1}{x^2 + 1} \;dx= -\int \dfrac{x}{x^2 + 1} + \dfrac{1}{x^2 + 1} \;dx= - \left( \frac{1}{2} \ln|x^2 + 1| + \arctan x \right) + K= -\frac{1}{2} \ln|x^2 + 1| - \arctan x + K
	\]



% 02/11
\checkin{02/11} 

























\end{document}